[chore] Brutally prune all oldlibs
Some more work needs done to present a clean theory of prime order
groups, and use it properly.

We should also ensure that we can eventually support DH over cyclic
groups of composite order (operating over prime order subgroups)

examples/Pedersen.ec
@@ -12,16 +12,15 @@
  *)
 require import Real.
 require import DLog.
-require import CyclicGroup.
 
 require (*--*) Commitment.
 
 (* Pedersen protocol types *)
 theory PedersenTypes.
   type value        = group.
-  type message      = F.t.
+  type message      = exp.
   type commitment   = group.
-  type openingkey   = F.t.
+  type openingkey   = exp.
 end PedersenTypes.
 export PedersenTypes.
 
@@ -36,14 +35,14 @@ export CommitmentProtocol.
 module Pedersen : CommitmentScheme = {
   proc gen() : value = {
     var x, h;
-    x <$ FDistr.dt;
+    x <$ dunifin;
     h <- g^x;
     return h;
   }
 
   proc commit(h: value, m: message) : commitment * openingkey = {
     var c, d;
-    d <$ FDistr.dt;
+    d <$ dunifin;
     c <- (g^d) * (h^m);
     return (c, d);
   }
@@ -57,7 +56,7 @@ module Pedersen : CommitmentScheme = {
 
 
 module DLogAttacker(B:Binder) : DLog.Adversary = {
-  proc guess(h: group) : F.t option = {
+  proc guess(h: group) : exp option = {
 
     var x, c, m, m', d, d';
     (c, m, d, m', d') <@ B.bind(h);
@@ -80,14 +79,14 @@ section PedersenSecurity.
   local module FakeCommit(U:Unhider) = {
     proc main() : bool = {
       var b, b', x, h, c, d;
-      var m0, m1 : F.t;
+      var m0, m1 : exp;
 
       (* Clearly, there are many useless lines, but their presence helps for the proofs *)
-      x <$ FDistr.dt;
+      x <$ dunifin;
       h <- g^x;
       (m0, m1) <@ U.choose(h);
       b <$ {0,1};
-      d <$ FDistr.dt;
+      d <$ dunifin;
       c <- g^d; (* message independent - fake commitment *)
       b' <@ U.guess(c);
 
@@ -100,7 +99,7 @@ section PedersenSecurity.
     islossless U.guess =>
     islossless FakeCommit(U).main.
   proof.
-    by move => uc_ll ug_ll; islossless; (apply FDistr.dt_ll || apply DBool.dbool_ll).
+    by move => uc_ll ug_ll; islossless.
   qed.
 
   (* Perfect hiding *)
@@ -113,7 +112,7 @@ section PedersenSecurity.
     proc; wp.
     swap 4 3.
     rnd (pred1 b'); call ug_ll; wp; rnd; call uc_ll; auto => />.
-    by rewrite FDistr.dt_ll /= => v _ _ result; rewrite DBool.dbool1E.
+    by rewrite dunifin_ll /= => v _ _ result; rewrite DBool.dbool1E.
   qed.
 
   local lemma phi_hi (U<:Unhider) &m:
@@ -122,10 +121,11 @@ section PedersenSecurity.
   proof.
     byequiv => //.
     proc; inline*.
-    call (_:true); wp.
+    call (: true); wp.
     rnd (fun d, (d + x * (b?m1:m0)){2})
         (fun d, (d - x * (b?m1:m0)){2}).
-    by wp; rnd; call (_: true); auto => />; progress; algebra.
+    wp; rnd; call (: true); auto=> />; progress; first 2 by ring.
+    by rewrite -expM -expD.
   qed.
 
   (* Perfect hiding - QED *)
@@ -150,7 +150,8 @@ section PedersenSecurity.
     + by split => [<- | ->]; field; apply: contra m_neq_m' => heq;ring heq.
     have -> : d - d' = x * (m' - m) <=> d + x * m = d' + x * m'.
     + by split => heq; ring heq.
-    by rewrite pow_bij -!(mul_pow, pow_pow, comm, comm').
+    move: comm'; rewrite comm -!expM -!expD=> /(congr1 loge).
+    by rewrite !loggK.
   qed.
 
   (*
