theories/crypto/DLog.ec
@@ -6,21 +6,34 @@
 
 (* A formalisation of the discrete logarithm assumption. *)
 
-require import CyclicGroup.
-require import Real.
+require import IntDiv Real.
 
+(** The group **)
+require (*--*) Group.
+
+clone export Group.CyclicGroup.
+
+(* The group has prime order *)
+axiom prime_order: prime order.
+
+clone export PowZMod
+proof
+  prime_order by rewrite prime_order.
+export ZModE ZModE.DZmodP.
+
+(** Discrete logarithm in a prime order cyclic group **)
 theory DLog.
 
   (* This is the standard definition of discrete logarithm experiment *)
   module type StdAdversary = {
-    proc guess(h : group) : F.t
+    proc guess(h : group) : exp
   }.
 
-  module DLogStdExperiment(A:StdAdversary) = {
+  module DLogStdExperiment (A:StdAdversary) = {
     proc main () : bool = {
       var x, x';
 
-      x  <$ FDistr.dt;
+      x  <$ dunifin;
       x' <@ A.guess(g^x);
 
       return (x' = x);
@@ -35,19 +48,19 @@ theory DLog.
      in the security parameter.
   *)
   module type Adversary = {
-    proc guess(h : group) : F.t option
+    proc guess(h : group) : exp option
   }.
 
-  module DLogExperiment(A:Adversary) = {
+  module DLogExperiment (A : Adversary) = {
     proc main () : bool = {
       var x, x';
 
-      x  <$ FDistr.dt;
+      x  <$ dunifin;
       x' <@ A.guess(g^x);
       return (x' = Some x);
     }
   }.
-  
+
 end DLog.
 
 (*
@@ -55,31 +68,30 @@ end DLog.
 *)
 section DLogSecurity.
 
-  declare module L <: DLog.Adversary.
+declare module L <: DLog.Adversary.
 
-  module StdRedAdversary(L:DLog.Adversary) = {
-    proc guess(h: group) : F.t = {
-      var lx, x;
+module StdRedAdversary (L : DLog.Adversary) = {
+  proc guess(h: group) : exp = {
+    var lx, x;
 
-      lx <@ L.guess(h);
-      if (lx = None)
-        x <$ FDistr.dt; (* the best if L gave up *)
-      else
-        x <- oget lx;
-
-      return x;
+    lx <@ L.guess(h);
+    if (lx = None) {
+      x <$ dunifin; (* the best if L gave up *)
+    } else {
+      x <- oget lx;
     }
-  }.
 
-  lemma dlog_standard_reduction &m:
-    Pr[DLog.DLogExperiment(L).main() @ &m : res] <=
-    Pr[DLog.DLogStdExperiment(StdRedAdversary(L)).main() @ &m : res].
-  proof.
-    byequiv => //; proc; inline*.
-    wp; seq 2 3: (x'{1} = lx{2} /\ x{1} = x{2}).
-    + by call (_: true); auto. 
-    if{2} => //; last by auto. 
-    auto => />; apply FDistr.dt_ll.
-  qed.
+    return x;
+  }
+}.
 
+lemma dlog_standard_reduction &m:
+  Pr[DLog.DLogExperiment(L).main() @ &m : res] <=
+  Pr[DLog.DLogStdExperiment(StdRedAdversary(L)).main() @ &m : res].
+proof.
+byequiv => //; proc; inline *.
+wp; seq 2 3: (x'{1} = lx{2} /\ x{1} = x{2}).
++ by call (_: true); auto.
+by if {2}; auto.
+qed.
 end section DLogSecurity.
